Blase/BlaseTest/Bool.lean
@@ -3,5 +3,5 @@ open BitVec
 
 theorem bool1 (x : Bool) : x = x := by bv_multi_width
 
-theorem bool2 (x y : Bool) (h : x = true ) : x = true := by
+theorem bool2 (x y : Bool) (h : x = true ) : true = x := by
   bv_multi_width +verbose?
